Finish fixing MinimunLogic.

GeneralLogic/Complete/ContextProperty.v
@@ -11,11 +11,29 @@ Context {L: Language}.
 Definition at_least (P cP: context -> Prop): Prop :=
   forall (Phi: context), cP Phi -> P Phi.
 
+Lemma at_least_self: forall P, at_least P P.
+Proof.
+  intros.
+  hnf; intros.
+  auto.
+Qed.
+
+Lemma at_least_left: forall P cP1 cP2, at_least P cP1 -> at_least P (Intersection _ cP1 cP2).
+Proof.
+  intros.
+  hnf in H |- *; intros.
+  destruct H0; auto.
+Qed.
+
+Lemma at_least_right: forall P cP1 cP2, at_least P cP2 -> at_least P (Intersection _ cP1 cP2).
+Proof.
+  intros.
+  hnf in H |- *; intros.
+  destruct H0; auto.
+Qed.
+
 Definition maximal (P: context -> Prop): context -> Prop :=
   fun Phi => P Phi /\ forall Psi, P Psi -> Included _ Phi Psi -> Included _ Psi Phi.
-
-Definition Lindenbaum_constructable (P cP: context -> Prop): Prop :=
-  forall Phi, P Phi -> exists Psi: sig cP, Included _ Phi (proj1_sig Psi) /\ P (proj1_sig Psi).
 
 Lemma sig_context_ext: forall (cP: context -> Prop) (Phi Psi: sig cP),
   (forall x, proj1_sig Phi x <-> proj1_sig Psi x) -> Phi = Psi.
@@ -31,5 +49,6 @@ Qed.
 
 End ContextProperty.
 
-
+Ltac solve_at_least :=
+  solve [apply at_least_self | auto | apply at_least_left; solve_at_least | apply at_least_right; solve_at_least].
 
