MinimunLogic/DeepEmbedded/Complete_Kripke.v
@@ -1,5 +1,6 @@
 Require Import Coq.Logic.Classical_Prop.
 Require Import Logic.lib.Ensembles_ext.
+Require Import Logic.lib.EnsemblesProperties.
 Require Import Logic.lib.Bijection.
 Require Import Logic.lib.Countable.
 Require Import Logic.GeneralLogic.Base.
@@ -10,24 +11,21 @@ Require Import Logic.GeneralLogic.Complete.ContextProperty.
 Require Import Logic.GeneralLogic.Complete.ContextProperty_Kripke.
 Require Import Logic.GeneralLogic.Complete.Lindenbaum.
 Require Import Logic.GeneralLogic.Complete.Canonical_Kripke.
+Require Import Logic.GeneralLogic.Complete.Complete_Kripke.
 Require Import Logic.MinimunLogic.Syntax.
 Require Import Logic.MinimunLogic.ProofTheory.Minimun2.
 Require Import Logic.MinimunLogic.Semantics.Kripke.
 Require Import Logic.MinimunLogic.Complete.ContextProperty_Kripke.
 Require Import Logic.MinimunLogic.Complete.Truth_Kripke.
-Require Import Logic.PropositionalLogic.Complete.Complete_Kripke.
-Require Logic.PropositionalLogic.DeepEmbedded.PropositionalLanguage.
-Require Logic.PropositionalLogic.DeepEmbedded.IntuitionisticLogic.
-Require Logic.PropositionalLogic.DeepEmbedded.DeMorganLogic.
-Require Logic.PropositionalLogic.DeepEmbedded.GodelDummettLogic.
-Require Logic.PropositionalLogic.DeepEmbedded.ClassicalLogic.
-Require Logic.PropositionalLogic.DeepEmbedded.KripkeSemantics.
+Require Import Logic.MinimunLogic.Complete.Lindenbaum_Kripke.
+Require Logic.MinimunLogic.DeepEmbedded.MinimunLanguage.
+Require Logic.MinimunLogic.DeepEmbedded.MinimunLogic.
+Require Logic.MinimunLogic.DeepEmbedded.KripkeSemantics.
 
 Local Open Scope logic_base.
 Local Open Scope syntax.
 Local Open Scope kripke_model.
 Local Open Scope kripke_model_class.
-Import PropositionalLanguageNotation.
 Import KripkeModelFamilyNotation.
 Import KripkeModelNotation_Intuitionistic.
 Import KripkeModelClass.
@@ -36,58 +34,46 @@ Section Complete.
 
 Context (Var: Type) (CV: Countable Var).
 
-Instance L: Language := PropositionalLanguage.L Var.
-Instance nL: NormalLanguage L := PropositionalLanguage.nL Var.
-Instance pL: PropositionalLanguage L := PropositionalLanguage.pL Var.
+Instance L: Language := MinimunLanguage.L Var.
+Instance minL: MinimunLanguage L := MinimunLanguage.minL Var.
 
-Instance Intuitionistic_G: ProofTheory L := IntuitionisticLogic.G Var.
-Instance DeMorgan_G: ProofTheory L := DeMorganLogic.G Var.
-Instance GodelDummett_G: ProofTheory L := GodelDummettLogic.G Var.
-Instance Classical_G: ProofTheory L := ClassicalLogic.G Var.
+Instance G: ProofTheory L := MinimunLogic.G Var.
+Instance AX: NormalAxiomatization L G := MinimunLogic.AX Var.
+Instance minAX: MinimunAxiomatization L G := MinimunLogic.minAX Var.
+Instance SC: NormalSequentCalculus L G := MinimunLogic.SC Var.
+Instance bSC: BasicSequentCalculus L G := MinimunLogic.bSC Var.
+Instance minSC: MinimunSequentCalculus L G := MinimunLogic.minSC Var.
 Instance Kripke_MD: Model := KripkeSemantics.MD Var.
 Instance Kripke_kMD: KripkeModel Kripke_MD := KripkeSemantics.kMD Var.
 Instance Kripke_R (M: Kmodel): Relation (Kworlds M) := KripkeSemantics.R Var M.
 Instance Kripke_SM: Semantics L Kripke_MD := KripkeSemantics.SM Var.
-Instance Kripke_kpSM (M: Kmodel): KripkePropositionalSemantics L Kripke_MD M Kripke_SM := KripkeSemantics.kpSM Var M.
+Instance Kripke_kminSM (M: Kmodel): KripkeMinimunSemantics L Kripke_MD M Kripke_SM := KripkeSemantics.kminSM Var M.
 
-Section General_Completeness.
+Definition cP: context -> Prop := derivable_closed.
 
-Context {Gamma: ProofTheory L}
-        {nGamma: NormalProofTheory L Gamma}
-        {mpGamma: MinimunPropositionalLogic L Gamma}
-        {ipGamma: IntuitionisticPropositionalLogic L Gamma}.
+Lemma AL_DC: at_least derivable_closed cP.
+Proof. solve_at_least. Qed.
 
-Definition DDC: context -> Prop := fun Psi =>
-  derivable_closed Psi /\ orp_witnessed Psi /\ consistent Psi.
-
-Lemma DER: at_least_derivable_closed DDC.
-Proof. hnf; intros ? [? [? ?]]; auto. Qed.
-
-Lemma ORP: at_least_orp_witnessed DDC.
-Proof. hnf; intros ? [? [? ?]]; auto. Qed.
-
-Lemma CONSI: at_least_consistent DDC.
-Proof. hnf; intros ? [? [? ?]]; auto. Qed.
-
-Lemma LIN_DER: Linderbaum_derivable DDC.
+Lemma LIN_CD: forall x: expr, Lindenbaum_constructable (cannot_derive x) cP.
 Proof.
-  hnf; intros.
-  pose proof Lindenbaum_lemma
-    (PropositionalLanguage.formula_countable Var CV)  _ _ H
-  as [Psi [? [? ?]]].
-  exists (exist _ Psi H2); auto.
+  intros.
+  apply Lindenbaum_constructable_suffice; auto.
+  + apply MinimunLanguage.formula_countable; auto.
+  + apply Lindenbaum_preserves_cannot_derive.
+  + unfold cP.
+    apply Lindenbaum_cannot_derive_ensures_derivable_closed.
 Qed.
 
 Definition canonical_frame: KripkeSemantics.frame :=
-  KripkeSemantics.Build_frame (sig DDC) (fun a b => Included _ (proj1_sig a) (proj1_sig b)).
+  KripkeSemantics.Build_frame (sig cP) (fun a b => Included _ (proj1_sig a) (proj1_sig b)).
 
 Definition canonical_eval: Var -> KripkeSemantics.sem canonical_frame :=
-  fun p a => proj1_sig a (PropositionalLanguage.varp p).
+  fun p a => proj1_sig a (MinimunLanguage.varp p).
 
 Definition canonical_Kmodel: @Kmodel (KripkeSemantics.MD Var) (KripkeSemantics.kMD Var) :=
   KripkeSemantics.Build_Kmodel Var canonical_frame canonical_eval.
 
-Definition rel: bijection (Kworlds canonical_Kmodel) (sig DDC) := bijection_refl.
+Definition rel: bijection (Kworlds canonical_Kmodel) (sig cP) := bijection_refl.
 
 Definition H_R:
   forall m n Phi Psi, rel m Phi -> rel n Psi ->
@@ -104,111 +90,23 @@ Lemma TRUTH:
     (KRIPKE: canonical_Kmodel, m |= x <-> proj1_sig Phi x).
 Proof.
   induction x.
-  + exact (truth_lemma_andp DDC rel DER x1 x2 IHx1 IHx2).
-  + exact (truth_lemma_orp DDC rel DER ORP x1 x2 IHx1 IHx2).
-  + exact (truth_lemma_impp DDC rel H_R DER LIN_DER x1 x2 IHx1 IHx2).
-  + exact (truth_lemma_falsep DDC rel CONSI).
+  + exact (truth_lemma_impp cP rel H_R AL_DC LIN_CD x1 x2 IHx1 IHx2).
   + intros; change (m = Phi) in H; subst; reflexivity.
 Qed.
 
-End General_Completeness.
+Import Logic.MinimunLogic.DeepEmbedded.KripkeSemantics.
 
-Section Intuitionistic_Completeness.
-
-Instance Intuitionistic_nG: NormalProofTheory L Intuitionistic_G := IntuitionisticLogic.nG Var.
-Instance Intuitionistic_mpG: MinimunPropositionalLogic L Intuitionistic_G := IntuitionisticLogic.mpG Var.
-Instance Intuitionistic_ipG: IntuitionisticPropositionalLogic L Intuitionistic_G := IntuitionisticLogic.ipG Var.
-
-Import Logic.PropositionalLogic.DeepEmbedded.KripkeSemantics.
-
-Theorem complete_intuitionistic_Kripke_all:
-  strongly_complete Intuitionistic_G Kripke_SM
+Theorem complete_MinimunLogic_Kripke_all:
+  strongly_complete G Kripke_SM
     (KripkeModelClass _ (Kmodel_Monotonic + Kmodel_PreOrder)).
 Proof.
-  apply (@general_completeness _ _ _ _ _ _ _ _ _ _ DDC rel LIN_DER DER TRUTH).
+  apply (general_completeness cP rel LIN_CD TRUTH).
   constructor; hnf.
   + intros.
-    exact (denote_monotonic DDC rel H_R
-             (PropositionalLanguage.varp v)
-             (TRUTH (PropositionalLanguage.varp v))).
-  + exact (po_R DDC rel H_R).
+    exact (denote_monotonic cP rel H_R
+             (MinimunLanguage.varp v)
+             (TRUTH (MinimunLanguage.varp v))).
+  + exact (po_R cP rel H_R).
 Qed.
-
-End Intuitionistic_Completeness.
-  
-Section DeMorgan_Completeness.
-
-Instance DeMorgan_nG: NormalProofTheory L DeMorgan_G := DeMorganLogic.nG Var.
-Instance DeMorgan_mpG: MinimunPropositionalLogic L DeMorgan_G := DeMorganLogic.mpG Var.
-Instance DeMorgan_ipG: IntuitionisticPropositionalLogic L DeMorgan_G := DeMorganLogic.ipG Var.
-Instance DeMorgan_dmpG: DeMorganPropositionalLogic L DeMorgan_G := DeMorganLogic.dmpG Var.
-
-Import Logic.PropositionalLogic.DeepEmbedded.KripkeSemantics.
-
-Theorem complete_DeMorgan_Kripke_branch_join:
-  strongly_complete DeMorgan_G Kripke_SM
-    (KripkeModelClass _ (Kmodel_Monotonic + Kmodel_PreOrder + Kmodel_BranchJoin)).
-Proof.
-  apply (@general_completeness _ _ _ _ _ _ _ _ _ _ DDC rel LIN_DER DER TRUTH).
-  constructor; [split |]; hnf.
-  + intros.
-    exact (denote_monotonic DDC rel H_R
-             (PropositionalLanguage.varp v)
-             (TRUTH (PropositionalLanguage.varp v))).
-  + exact (po_R DDC rel H_R).
-  + exact (DeMorgan_canonical_branch_join DDC rel H_R DER ORP CONSI LIN_DER).
-Qed.
-
-End DeMorgan_Completeness.
-
-Section GodelDummett_Completeness.
-
-Instance GodelDummett_nG: NormalProofTheory L GodelDummett_G := GodelDummettLogic.nG Var.
-Instance GodelDummett_mpG: MinimunPropositionalLogic L GodelDummett_G := GodelDummettLogic.mpG Var.
-Instance GodelDummett_ipG: IntuitionisticPropositionalLogic L GodelDummett_G := GodelDummettLogic.ipG Var.
-Instance GodelDummett_gdpG: GodelDummettPropositionalLogic L GodelDummett_G := GodelDummettLogic.gdpG Var.
-
-Import Logic.PropositionalLogic.DeepEmbedded.KripkeSemantics.
-
-Theorem complete_GodelDummett_Kripke_no_branch:
-  strongly_complete GodelDummett_G Kripke_SM
-    (KripkeModelClass _ (Kmodel_Monotonic + Kmodel_PreOrder + Kmodel_NoBranch)).
-Proof.
-  apply (@general_completeness _ _ _ _ _ _ _ _ _ _ DDC rel LIN_DER DER TRUTH).
-  constructor; [split |]; hnf.
-  + intros.
-    exact (denote_monotonic DDC rel H_R
-             (PropositionalLanguage.varp v)
-             (TRUTH (PropositionalLanguage.varp v))).
-  + exact (po_R DDC rel H_R).
-  + exact (GodelDummett_canonical_no_branch DDC rel H_R DER ORP).
-Qed.
-
-End GodelDummett_Completeness.
-
-Section Classical_Completeness.
-
-Instance Classical_nG: NormalProofTheory L Classical_G := ClassicalLogic.nG Var.
-Instance Classical_mpG: MinimunPropositionalLogic L Classical_G := ClassicalLogic.mpG Var.
-Instance Classical_ipG: IntuitionisticPropositionalLogic L Classical_G := ClassicalLogic.ipG Var.
-Instance Classical_cpG: ClassicalPropositionalLogic L Classical_G := ClassicalLogic.cpG Var.
-
-Import Logic.PropositionalLogic.DeepEmbedded.KripkeSemantics.
-
-Theorem complete_Classical_Kripke_identity:
-  strongly_complete Classical_G Kripke_SM
-    (KripkeModelClass _ (Kmodel_Monotonic + Kmodel_PreOrder + Kmodel_Identity)).
-Proof.
-  apply (@general_completeness _ _ _ _ _ _ _ _ _ _ DDC rel LIN_DER DER TRUTH).
-  constructor; [split |]; hnf.
-  + intros.
-    exact (denote_monotonic DDC rel H_R
-             (PropositionalLanguage.varp v)
-             (TRUTH (PropositionalLanguage.varp v))).
-  + exact (po_R DDC rel H_R).
-  + exact (classical_canonical_ident DDC rel H_R DER ORP CONSI).
-Qed.
-
-End Classical_Completeness.
 
 End Complete.
