GeneralLogic/Complete/Complete_Kripke.v
@@ -7,6 +7,7 @@ Require Import Logic.GeneralLogic.Base.
 Require Import Logic.GeneralLogic.KripkeModel.
 Require Import Logic.GeneralLogic.ProofTheory.BasicSequentCalculus.
 Require Import Logic.GeneralLogic.Semantics.Kripke.
+Require Import Logic.GeneralLogic.Complete.Lindenbaum.
 Require Import Logic.GeneralLogic.Complete.ContextProperty.
 Require Import Logic.GeneralLogic.Complete.ContextProperty_Kripke.
 
