MinimunLogic/Complete/Lindenbaum_Kripke.v
@@ -4,23 +4,41 @@ Require Import Coq.Logic.Classical_Pred_Type.
 Require Import Logic.lib.Bijection.
 Require Import Logic.lib.Countable.
 Require Import Logic.GeneralLogic.Base.
-Require Import Logic.GeneralLogic.KripkeModel.
+Require Import Logic.GeneralLogic.ProofTheory.BasicSequentCalculus.
+Require Import Logic.GeneralLogic.Complete.Lindenbaum.
+Require Import Logic.GeneralLogic.Complete.Lindenbaum_Kripke.
+Require Import Logic.GeneralLogic.Complete.ContextProperty.
+Require Import Logic.GeneralLogic.Complete.ContextProperty_Kripke.
+Require Import Logic.MinimunLogic.Syntax.
+Require Import Logic.MinimunLogic.ProofTheory.Minimun2.
 Require Import Logic.MinimunLogic.Complete.ContextProperty_Kripke.
 
 Local Open Scope logic_base.
 Local Open Scope kripke_model.
 Import KripkeModelFamilyNotation.
-Import KripkeModelNotation_Intuitionistic.
 
 Section Lindenbaum_Kripke.
 
 Context {L: Language}
-        {Gamma: ProofTheory L}.
+        {minL: MinimunLanguage L}
+        {Gamma: ProofTheory L}
+        {AX: NormalAxiomatization L Gamma}
+        {bSC: BasicSequentCalculus L Gamma}.
 
-Hypothesis CE: Countable expr.
+Lemma Lindenbaum_preserves_cannot_derive: forall x, Lindenbaum_preserves (cannot_derive x).
+Proof.
+  intros.
+  apply Lindenbaum_preserves_by_finiteness.
+  - apply cannot_derive_finite_captured.
+  - apply cannot_derive_subset_preserved.
+Qed.
 
-Lemma Lindenbaum_constructable_DS: forall P,
-  
-    Lindenbaum_constructable P derivable_closed.
+Lemma Lindenbaum_cannot_derive_ensures_derivable_closed: forall x, Lindenbaum_ensures (cannot_derive x) derivable_closed.
+Proof.
+  intros.
+  apply Lindenbaum_for_derivable_closed.
+  - apply Lindenbaum_preserves_cannot_derive.
+  - apply cannot_derive_derivable_subset_preserved.
+Qed.
 
 End Lindenbaum_Kripke.
