MinimunLogic/Complete/Truth_Kripke.v
@@ -9,6 +9,7 @@ Require Import Logic.GeneralLogic.KripkeModel.
 Require Import Logic.GeneralLogic.Semantics.Kripke.
 Require Import Logic.GeneralLogic.Complete.ContextProperty.
 Require Import Logic.GeneralLogic.Complete.ContextProperty_Kripke.
+Require Import Logic.GeneralLogic.Complete.Lindenbaum.
 Require Import Logic.MinimunLogic.Syntax.
 Require Import Logic.MinimunLogic.ProofTheory.Minimun2.
 Require Import Logic.MinimunLogic.Semantics.Kripke.
@@ -39,8 +40,8 @@ Context (cP: context -> Prop)
 Hypothesis H_R: forall m n Phi Psi, rel m Phi -> rel n Psi -> (m <= n <-> Included _ (proj1_sig Phi) (proj1_sig Psi)).
 
 Lemma truth_lemma_impp
-      (DER: at_least derivable_closed cP)
-      (LIN_DER: forall x, Lindenbaum_constructable (cannot_derive x) cP)
+      (AL_DC: at_least derivable_closed cP)
+      (LIN_CD: forall x, Lindenbaum_constructable (cannot_derive x) cP)
       (x y: expr)
       (IHx: forall m Phi, rel m Phi -> (KRIPKE: M, m |= x <-> proj1_sig Phi x))
       (IHy: forall m Phi, rel m Phi -> (KRIPKE: M, m |= y <-> proj1_sig Phi y)):
@@ -49,17 +50,17 @@ Proof.
   intros.
   rewrite sat_impp.
   split; intros.
-  + rewrite derivable_closed_element_derivable by (apply DER, (proj2_sig Phi)).
+  + rewrite derivable_closed_element_derivable by (apply AL_DC, (proj2_sig Phi)).
     rewrite <- deduction_theorem.
     apply NNPP; intro.
-    apply LIN_DER in H1.
+    apply LIN_CD in H1.
     destruct H1 as [Psi [? ?]].
     apply H2; clear H2.
     assert (Included _ (proj1_sig Phi) (proj1_sig Psi)) by (intros ? ?; apply H1; left; auto).
     assert (proj1_sig Psi x) by (apply H1; right; constructor; auto).
     clear H1.
     destruct (su_bij _ _ rel Psi) as [n ?].
-    rewrite <- derivable_closed_element_derivable by (apply DER, (proj2_sig Psi)).
+    rewrite <- derivable_closed_element_derivable by (apply AL_DC, (proj2_sig Psi)).
     rewrite <- (IHx _ _ H1) in H3.
     rewrite <- (IHy _ _ H1).
     apply H0; auto.
@@ -68,9 +69,9 @@ Proof.
   + destruct (im_bij _ _ rel n) as [Psi ?].
     rewrite (IHx _ _ H3) in H2.
     rewrite (IHy _ _ H3).
-    rewrite derivable_closed_element_derivable in H2 |- * by (apply DER, (proj2_sig Psi)).
+    rewrite derivable_closed_element_derivable in H2 |- * by (apply AL_DC, (proj2_sig Psi)).
     eapply deduction_modus_ponens; [exact H2 |].
-    rewrite <- derivable_closed_element_derivable by (apply DER, (proj2_sig Psi)).
+    rewrite <- derivable_closed_element_derivable by (apply AL_DC, (proj2_sig Psi)).
     erewrite H_R in H1 by eauto.
     apply H1; auto.
 Qed.
